dimsum/iris/iris.v
@@ -1,0 +1,4 @@
+From dimsum.core Require Export module trefines.
+From dimsum.core.iris Require Export sim.
+
+(** This file reexports all relevant modules and should be imported by clients. *)
