dimsum/nb_mod.v
@@ -1,0 +1,16 @@
+From dimsum.core Require Export module trefines.
+
+Definition nb_step EV (_ : unit) (_ : option EV) (_ : unit → Prop) : Prop := False.
+Definition nb_trans EV : mod_trans EV := ModTrans (nb_step EV).
+Definition nb_mod EV : module EV := Mod (nb_trans EV) tt.
+
+Lemma nb_trans_has_trace EV σ κ Pσ :
+  σ ~{ nb_trans EV, option_trace κ }~>ₜ Pσ →
+  κ = None ∧ Pσ tt.
+Proof.
+  move => Ht. destruct κ, σ.
+  - apply thas_trace_cons_inv in Ht.
+    apply thas_trace_nil_inv in Ht. inv Ht => //. destruct!.
+    inv_all @m_step.
+  - apply thas_trace_nil_inv in Ht. by inv Ht.
+Qed.
